spot/GC.SPOT.ThreeObjects.fsti
@@ -1,0 +1,115 @@
+module GC.SPOT.ThreeObjects
+
+open FStar.Seq
+module Seq = FStar.Seq
+module U64 = FStar.UInt64
+
+open GC.Spec.Base
+open GC.Gen.Base
+open GC.Gen.MinorHeap
+
+val spot_roots : c:obj_addr -> Tot (seq U64.t)
+
+val spot_c_to_a_slot
+  : c:obj_addr{U64.v c + GC.SPOT.Layout.c_to_a_field_index * 8 + 8 <= heap_size} ->
+    Tot hp_addr
+
+val spot_slots
+  : c:obj_addr{U64.v c + GC.SPOT.Layout.c_to_a_field_index * 8 + 8 <= heap_size} ->
+    Tot (seq U64.t)
+
+val spot_roots_mem_c
+  : c:obj_addr -> Lemma (Seq.mem (c <: U64.t) (spot_roots c))
+
+val spot_roots_mem_a
+  : c:obj_addr -> Lemma (Seq.mem GC.SPOT.Layout.a_minor (spot_roots c))
+
+val spot_slots_singleton_distinct
+  : c:obj_addr{U64.v c + GC.SPOT.Layout.c_to_a_field_index * 8 + 8 <= heap_size} ->
+    Lemma (GC.Gen.Impl.UpdatePtrs.slots_pairwise_distinct (spot_slots c) 1)
+
+val spot_minor_scenario_pre
+  : minor:minor_state -> major:heap -> fp:U64.t ->
+    c:obj_addr{U64.v c + GC.SPOT.Layout.c_to_a_field_index * 8 + 8 <= heap_size} ->
+    farr:seq U64.t -> Tot prop
+
+val spot_full_scenario_pre
+  : minor:minor_state -> major:heap -> fp:U64.t ->
+    c:obj_addr{U64.v c + GC.SPOT.Layout.c_to_a_field_index * 8 + 8 <= heap_size} ->
+    farr:seq U64.t -> st:seq obj_addr -> cap:nat -> Tot prop
+
+val spot_c_reachable_root
+  : minor:minor_state -> major:heap -> fp:U64.t ->
+    c:obj_addr{U64.v c + GC.SPOT.Layout.c_to_a_field_index * 8 + 8 <= heap_size} ->
+    farr:seq U64.t ->
+    Lemma
+      (requires spot_minor_scenario_pre minor major fp c farr)
+      (ensures (
+        let cg = GC.Gen.CombinedGraph.build_combined_graph minor major in
+        GC.Gen.CombinedGraph.combined_reachable
+          cg (GC.Gen.CombinedGraph.classify_roots (spot_roots c))
+          (GC.Gen.CombinedGraph.MajorV c)))
+
+val spot_a_reachable_root
+  : minor:minor_state -> major:heap -> fp:U64.t ->
+    c:obj_addr{U64.v c + GC.SPOT.Layout.c_to_a_field_index * 8 + 8 <= heap_size} ->
+    farr:seq U64.t ->
+    Lemma
+      (requires spot_minor_scenario_pre minor major fp c farr)
+      (ensures (
+        let cg = GC.Gen.CombinedGraph.build_combined_graph minor major in
+        GC.Gen.CombinedGraph.combined_reachable
+          cg (GC.Gen.CombinedGraph.classify_roots (spot_roots c))
+          (GC.Gen.CombinedGraph.MinorV GC.SPOT.Layout.a_minor)))
+
+val spot_a_promoted
+  : minor:minor_state -> major:heap -> fp:U64.t ->
+    c:obj_addr{U64.v c + GC.SPOT.Layout.c_to_a_field_index * 8 + 8 <= heap_size} ->
+    farr:seq U64.t ->
+    Lemma
+      (requires spot_minor_scenario_pre minor major fp c farr)
+      (ensures (
+        let prom = GC.Gen.Cheney.cheney_promote minor major fp (spot_roots c) in
+        GC.SPOT.Postconditions.promoted_image
+          minor major fp (spot_roots c) GC.SPOT.Layout.a_minor
+          (prom.fwd_map GC.SPOT.Layout.a_minor)))
+
+val spot_c_field_rewritten_to_a_prime
+  : minor:minor_state -> major:heap -> fp:U64.t ->
+    c:obj_addr{U64.v c + GC.SPOT.Layout.c_to_a_field_index * 8 + 8 <= heap_size} ->
+    farr:seq U64.t ->
+    Lemma
+      (requires spot_minor_scenario_pre minor major fp c farr)
+      (ensures (
+        let prom = GC.Gen.Cheney.cheney_promote minor major fp (spot_roots c) in
+        let res = GC.Gen.Cheney.cheney_collect_spec minor major fp (spot_roots c) in
+        GC.SPOT.Postconditions.promoted_image
+          minor major fp (spot_roots c) GC.SPOT.Layout.a_minor
+          (prom.fwd_map GC.SPOT.Layout.a_minor) /\
+        GC.Spec.Heap.read_word res.mc_major (spot_c_to_a_slot c) ==
+          prom.fwd_map GC.SPOT.Layout.a_minor))
+
+val spot_b_not_promoted_from_forwarding_zero
+  : minor:minor_state -> major:heap -> fp:U64.t -> c:obj_addr ->
+    Lemma
+      (requires
+        (GC.Gen.Cheney.cheney_promote minor major fp (spot_roots c)).fwd_map
+          GC.SPOT.Layout.b_minor == 0UL)
+      (ensures
+        GC.SPOT.Postconditions.minor_not_promoted
+          minor major fp (spot_roots c) GC.SPOT.Layout.b_minor)
+
+val spot_final_survives_from_gen_gc_post
+  : minor:minor_state -> major:heap -> fp:U64.t ->
+    c:obj_addr{U64.v c + GC.SPOT.Layout.c_to_a_field_index * 8 + 8 <= heap_size} ->
+    roots_out:seq U64.t -> ok:bool -> final_major:heap -> st:seq obj_addr ->
+    x:obj_addr ->
+    Lemma
+      (requires
+        ok /\
+        GC.Gen.Impl.gen_gc_reachable_subgraph_isomorphism_post
+          minor major fp (spot_roots c) ok final_major roots_out st /\
+        GC.Spec.Correctness.heap_reachable
+          (GC.Gen.Cheney.cheney_collect_spec minor major fp (spot_roots c)).mc_major
+          st x)
+      (ensures Seq.mem x (GC.Spec.Fields.objects zero_addr final_major))
